in-place linked list reversal

LiveVerif/src/LiveVerifExamples/linked_list.v
@@ -1,3 +1,4 @@
+(* -*- eval: (load-file "../LiveVerif/live_verif_setup.el"); -*- *)
 Require Import LiveVerif.LiveVerifLib.
 Require Import coqutil.Tactics.syntactic_unify.
 Require Import Lia.
@@ -65,23 +66,124 @@ Derive malloc_node SuchThat (fun_correct! malloc_node) As malloc_node_ok. .**/
   unfold seps. unfold iff1. unfold emp. intuition.
 Qed.
 
-
 Fixpoint sll (L : list word) (p : word): mem -> Prop :=
   match L with
   | nil => emp (p = /[0])
-  | x::L' => ex1 (fun (q:word) =>
-      <{ * uintptr x p
+  | x::L' => ex1 (fun q =>
+         (* TODO maybe all judgments, including uintptr etc, should enforce pointers
+            to be non-NULL? *)
+      <{ * emp (p <> /[0])
+         * uintptr x p
          * uintptr q (p ^+ /[4])
          * sll L' q }>)
   end.
 
-Lemma purify_sll:
-  forall L p,
-    purify (sll L p) (True).
+Lemma purify_sll: forall L p, purify (sll L p) True.
 Proof.
   unfold purify. auto.
 Qed.
-Hint Resolve purify_sll : purify.
+Hint Resolve purify_sll | 5 : purify.
+
+Local Hint Extern 1 (PredicateSize (sll ?l)) =>
+  let r := eval cbv iota in
+    (match l with
+     | cons _ _ => 8
+     | nil => 0
+     end) in
+  exact r
+: typeclass_instances.
+
+Lemma invert_sll_null: forall l m, m |= sll l /[0] -> m |= emp (l = nil).
+Proof.
+  unfold with_mem. intros. destruct l; simpl in *.
+  - unfold emp in *. destruct H. auto.
+  - destruct H as [q H]. repeat heapletwise_step. congruence.
+Qed.
+
+Lemma invert_sll_nonnull: forall l m p, p <> /[0] -> sll l p m -> exists x l' q,
+  l = x :: l' /\
+  <{ * uintptr x p
+     * uintptr q (p ^+ /[4])
+     * sll l' q }> m.
+Proof.
+  intros. destruct l.
+  - simpl in *. eapply purify_emp in H0. congruence.
+  - simpl in *. destruct H0 as [q M]. eapply sep_emp_l in M. apply proj2 in M. eauto.
+Qed.
+
+Lemma fold_sll_cons: forall p, p <> /[0] -> forall x q l m,
+  <{ * uintptr x p
+     * uintptr q (p ^+ /[4])
+     * sll l q }> m ->
+  sll (cons x l) p m.
+Proof.
+  intros. simpl. unfold ex1. exists q.
+  eapply sep_emp_l. auto.
+Qed.
+
+(* even though in-place, memory cell containing the head of the element will change,
+   so it returns a pointer to the new head of the list (which used to be its last cell) *)
+#[export] Instance spec_of_sll_reverse: fnspec := .**/
+
+uintptr_t sll_reverse(uintptr_t p) /**#
+  ghost_args := (l : list word) (R: mem -> Prop);
+  requires t m := <{ * sll l p
+                     * R }> m;
+  ensures t' m' r := t' = t /\
+       <{ * sll (List.rev l) r
+          * R }> m' #**/ /**.
+Derive sll_reverse SuchThat (fun_correct! sll_reverse) As sll_reverse_ok.       .**/
+{                                                                          /**. .**/
+  uintptr_t acc = 0;                                                       /**.
+
+  pose (lDone := @nil word).
+  pose (lTodo := l).
+  prove (l = lDone ++ lTodo). { reflexivity. }
+  move H before acc.
+  swap l with lTodo in #(sll l p).
+  swap R with (sep (sll (List.rev lDone) acc) R) in #R.
+  { subst lDone. simpl. eapply iff1ToEq.
+    step. cancel. simpl. unfold emp, iff1. intuition idtac. }
+  unfold with_mem in H1.
+  repeat heapletwise_step.
+  clearbody lDone. clearbody lTodo.
+  loop invariant above acc.
+  move p after acc.
+  delete #(acc = ??).
+
+  (* TODO != operator *)                                                        .**/
+  while (!(p == 0)) /* decreases (len lTodo) */ {                          /**.
+
+    match goal with
+    | H: _ |= sll lTodo p |- _ => rename H into HT
+    end.
+    eapply invert_sll_nonnull in HT. 2: assumption. fwd. repeat heapletwise_step.
+                                                                                .**/
+    uintptr_t tail = load(p + 4);                                          /**. .**/
+    store(p + 4, acc);                                                     /**.
+
+    epose proof (fold_sll_cons _ #(p <> /[0])) as HL.
+    cancel_in_hyp HL.
+    rewrite <- List.rev_unit in HL.
+                                                                                .**/
+    acc = p;                                                               /**. .**/
+    p = tail;                                                              /**. .**/
+  }                                                                        /*?.
+
+step. step. step. step. step. step. step. step. step. step. step. step.
+step. step.
+instantiate (1 := l').
+step. step. step. step. step. step. step. step. step. step. step. step. step.
+end while.
+                                                                                .**/
+  return acc;                                                              /**.
+
+  eapply invert_sll_null in H2.
+  repeat heapletwise_step. subst lTodo.
+  bottom_up_simpl_in_hyps. subst lDone.
+                                                                                .**/
+}                                                                          /**.
+Qed.
 
 #[export] Instance spec_of_sll_prepend: fnspec := .**/
 
